Progress on reworked ebfs phase proof

Layering_Algo.thy
@@ -152,34 +152,111 @@ definition ebfs_phase :: "_ graph \<Rightarrow> node set \<Rightarrow> (_ graph 
     })
     (c\<^sub>i, {})"
 
+definition ebfs_phase_invar :: "node \<Rightarrow> nat \<Rightarrow> _ graph \<Rightarrow> node set \<Rightarrow> (_ graph \<times> node set) \<Rightarrow> bool" where
+  "ebfs_phase_invar s n c\<^sub>i Q \<equiv> \<lambda>(c', Q').
+    CapacityCompatibleGraphs c' c
+    \<and> Graph.E c' = Graph.E c\<^sub>i \<union> (exactDistNodes n s - Q) \<times> Q'
+    \<and> Q' = exactDistNodes (Suc n) s \<inter> Graph.V c'"
 
-(* TODO from here *)
+lemma ebfs_phase_initial:
+  assumes "Bounded_S_Shortest_Path_Union c' c s V n"
+  shows "ebfs_phase_invar s n c' (exactDistNodes n s) (c', {})"
+  unfolding ebfs_phase_invar_def
+proof (intro case_prodI conjI)
+  from assms interpret Bounded_S_Shortest_Path_Union c' c s V n .
+
+  (* TODO improve by introducing distance bounded locale for Bounded_S_SPU*)
+  have "\<And>u. u \<in> V' \<Longrightarrow> min_dist s u \<le> n" using min_dist_transfer obtain_close_ST by auto
+  then show "{} = exactDistNodes (Suc n) s \<inter> Graph.V c'" unfolding exactDistNodes_def by fastforce
+  show "CapacityCompatibleGraphs c' c" by intro_locales
+  show "Graph.E c' = Graph.E c' \<union> (exactDistNodes n s - exactDistNodes n s) \<times> {}" by simp
+qed
+
+lemma ebfs_phase_final:
+  assumes BSPU: "Bounded_S_Shortest_Path_Union c\<^sub>i c s V n"
+    and INVAR: "ebfs_phase_invar s n c\<^sub>i {} (c', Q')"
+  shows "Bounded_S_Shortest_Path_Union c' c s V (Suc n) \<and> Q' = exactDistNodes (Suc n) s"
+proof
+  from INVAR have "CapacityCompatibleGraphs c' c"
+    and E': "Graph.E c' = Graph.E c\<^sub>i \<union> exactDistNodes n s \<times> Q'"
+    and Q': "Q' = exactDistNodes (Suc n) s \<inter> Graph.V c'"
+    unfolding ebfs_phase_invar_def by auto
+  then interpret CapacityCompatibleGraphs c' c by simp
+
+  show "Bounded_S_Shortest_Path_Union c' c s V (Suc n)"
+  proof
+    (*from BSPU interpret Bounded_S_Shortest_Path_Union c\<^sub>i c s V n .*)
+
+  qed
+  then have "exactDistNodes (Suc n) s \<subseteq> Graph.V c'" unfolding exactDistNodes_def sorry
+  then show "Q' = exactDistNodes (Suc n) s" using INVAR unfolding ebfs_phase_invar_def by fast
+qed
+
+
+
+
+
 (*
-definition ebfs_phase_invar :: "node \<Rightarrow> nat \<Rightarrow> node set \<Rightarrow> (_ graph \<times> node set) \<Rightarrow> bool" where
-  "ebfs_phase_invar s n Q \<equiv> \<lambda>(c', Q').
-    S_Shortest_Path_Union c' c s (boundedReachableNodes (Suc n) s - Q)
-    \<and> Q' = exactDistNodes (n + 2) s \<inter> {v. \<exists>u \<in> Graph.V c'. (u, v) \<in> E}"
+  from assms show "S_Shortest_Path_Union c' c s (boundedReachableNodes (Suc n) s)"
+    unfolding ebfs_phase_invar_def by simp
+  then interpret S_Shortest_Path_Union c' c s "boundedReachableNodes (Suc n) s" . (* TODO necessary? *)
+
+  from assms have "Q' = exactDistNodes (n + 2) s \<inter> {v. \<exists>u \<in> Graph.V c'. (u, v) \<in> E}"
+    unfolding ebfs_phase_invar_def by simp
+  moreover have "exactDistNodes (n + 2) s \<subseteq> {v. \<exists>u \<in> Graph.V c'. (u, v) \<in> E}"
+  proof (* TODO prettify *)
+    fix v
+    assume "v \<in> exactDistNodes (n + 2) s"
+    then obtain p where P: "isShortestPath s p v" "length p = n + 2" unfolding exactDistNodes_def
+      by (metis (mono_tags) isShortestPath_min_dist_def mem_Collect_eq obtain_shortest_path)
+    then obtain p\<^sub>u u where "p = p\<^sub>u @ [(u, v)]"
+      by (metis Graph.isPath_bwd_cases add_2_eq_Suc' isShortestPath_def length_Suc_conv list.distinct(1))
+    with P have "isShortestPath s p\<^sub>u u" "length p\<^sub>u = n + 1" "(u, v) \<in> E"
+      using split_shortest_path_around_edge 
+      by (metis Graph.isPath_tail add_Suc_right add_left_imp_eq length_append_singleton nat_1_add_1 plus_1_eq_Suc shortestPath_is_path)+
+    then have "u \<in> boundedReachableNodes (Suc n) s" unfolding boundedReachableNodes_def
+      by (metis connected_def Suc_eq_plus1 isShortestPath_def isShortestPath_min_dist_def mem_Collect_eq)
+    then have "u \<in> V'"
+      by (metis Graph.connected_edgeRtc Graph.connected_inV_iff Graph.distinct_nodes_in_V_if_connected(1) Graph.isPath_rtc Graph.isShortestPath_alt Graph.shortestPath_is_path Graph.simplePath_same_conv Suc_eq_plus1 \<open>isShortestPath s p\<^sub>u u\<close> \<open>length p\<^sub>u = n + 1\<close> insert_iff length_Suc_conv list.distinct(1) shortest_ST_path_remains)
+    with \<open>(u, v) \<in> E\<close> show "v \<in> {v. \<exists>u\<in>V'. (u, v) \<in> E}" by blast
+  qed
+  ultimately show "Q' = exactDistNodes (n + 2) s" by blast
+qed
 *)
 
-definition ebfs_phase_invar :: "node \<Rightarrow> nat \<Rightarrow> node set \<Rightarrow> (_ graph \<times> node set) \<Rightarrow> bool" where
-  "ebfs_phase_invar s n Q \<equiv> \<lambda>(c', Q').
-    CapacityCompatibleGraphs c' c
 
 
 
-    S_Shortest_Path_Union c' c s (boundedReachableNodes (Suc n) s - Q)
-    \<and> Q' = exactDistNodes (n + 2) s \<inter> {v. \<exists>u \<in> Graph.V c'. (u, v) \<in> E}"
+
+
+
 
 lemma ebfs_phase_correct:
   fixes s c' Q n
-  assumes "finite (reachableNodes s)" (*"finite (exactDistNodes n s)"*)
-    and "S_Shortest_Path_Union c' c s (boundedReachableNodes n s)"
-  shows "ebfs_phase c' (exactDistNodes n s) \<le> SPEC (\<lambda>(c'', Q'). S_Shortest_Path_Union c'' c s (boundedReachableNodes (Suc n) s) \<and> Q' = exactDistNodes (Suc n) s)"
+  assumes FIN: "finite (reachableNodes s)" (*"finite (exactDistNodes n s)"*)
+    and BSPU: "Bounded_S_Shortest_Path_Union c' c s V n"
+  shows "ebfs_phase c' (exactDistNodes n s) \<le> SPEC (\<lambda>(c'', Q'). Bounded_S_Shortest_Path_Union c'' c s V (Suc n) \<and> Q' = exactDistNodes (Suc n) s)"
   unfolding ebfs_phase_def
-  apply (refine_vcg FOREACH_rule[where I="ebfs_phase_invar s n"])
-  using assms finite_subset apply (metis Diff_subset exactDistNodes_alt boundedReachableNodes_ss)
+  apply (refine_vcg FOREACH_rule[where I="ebfs_phase_invar s n c'"])
+  using FIN finite_subset exactDistNodes_reachable_ss boundedReachableNodes_ss apply meson
+  using BSPU ebfs_phase_initial apply simp
+
+  using ebfs_phase_final[OF BSPU] apply simp_all
   using assms ebfs_phase_initial ebfs_phase_step ebfs_phase_final by simp_all
 
+
+(*
+lemma ebfs_phase_correct:
+  fixes s c' Q n
+  assumes FIN: "finite (reachableNodes s)" (*"finite (exactDistNodes n s)"*)
+    and SPU: "S_Shortest_Path_Union c' c s (boundedReachableNodes n s)"
+  shows "ebfs_phase c' (exactDistNodes n s) \<le> SPEC (\<lambda>(c'', Q'). S_Shortest_Path_Union c'' c s (boundedReachableNodes (Suc n) s) \<and> Q' = exactDistNodes (Suc n) s)"
+  unfolding ebfs_phase_def
+  apply (refine_vcg FOREACH_rule[where I="ebfs_phase_invar s n c'"])
+  using FIN finite_subset exactDistNodes_reachable_ss boundedReachableNodes_ss apply meson
+  using ebfs_phase_initial[OF SPU] apply simp
+  using assms ebfs_phase_initial ebfs_phase_step ebfs_phase_final by simp_all
+*)
 
 
 
@@ -358,6 +435,7 @@ proof -
 qed
 end
 
+(*
 lemma ebfs_phase_correct:
   fixes s c' Q n
   assumes "finite (reachableNodes s)" (*"finite (exactDistNodes (Suc n) s)"*)
@@ -365,8 +443,9 @@ lemma ebfs_phase_correct:
   shows "ebfs_phase c' (exactDistNodes (Suc n) s) \<le> SPEC(\<lambda>(c'', Q'). S_Shortest_Path_Union c'' c s (boundedReachableNodes (Suc n) s) \<and> Q' = exactDistNodes (n + 2) s)"
   unfolding ebfs_phase_def
   apply (refine_vcg FOREACH_rule[where I="ebfs_phase_invar s n"])
-  using assms finite_subset apply (metis Diff_subset exactDistNodes_alt boundedReachableNodes_ss)
+  using assms finite_subset sorry  apply (metis Diff_subset exactDistNodes_alt boundedReachableNodes_ss)
   using assms ebfs_phase_initial ebfs_phase_step ebfs_phase_final by simp_all
+*)
 
 thm FOREACH_rule
 (* TODO somewhere we need the fact that the set of reachable nodes (from s) is finite *)
